chore: Env -> Axioms

GroupoidModel/Syntax/Axioms.lean
@@ -1,7 +1,7 @@
 import GroupoidModel.Syntax.Synth
 import GroupoidModel.Syntax.Typechecker.Value
 
-variable {χ : Type*} {E : Env χ}
+variable {χ : Type*} {E : Axioms χ}
 
 theorem isClosed_all :
     (∀ {Γ l A}, E ∣ Γ ⊢[l] A → A.isClosed Γ.length) ∧
@@ -18,30 +18,30 @@ theorem WfTm.isClosed {l A t} : E ∣ [] ⊢[l] t : A → t.isClosed := isClosed
 
 /-! ## Constant environments -/
 
-namespace Env
+namespace Axioms
 
-def empty (χ) : Env χ := fun _ => none
+def empty (χ) : Axioms χ := fun _ => none
 
 theorem Wf.empty (χ) : (empty χ).Wf := nofun
 
 open Classical
 
-instance : LE (Env χ) where
+instance : LE (Axioms χ) where
   le E E' := ∀ ⦃c p⦄, (E c) = some p → (E' c) = some p
 
-noncomputable def snoc (E : Env χ)
+noncomputable def snoc (E : Axioms χ)
     (l : Nat) (c : χ) (A : Expr χ)
-    (l_le : l ≤ univMax) (A_cl : A.isClosed) : Env χ :=
+    (l_le : l ≤ univMax) (A_cl : A.isClosed) : Axioms χ :=
   fun d => if d = c then some ⟨(A, l), ⟨A_cl, l_le⟩⟩ else E d
 
 @[simp]
-theorem snoc_get (E : Env χ)
+theorem snoc_get (E : Axioms χ)
     (l : Nat) (c : χ) (A : Expr χ)
     (l_le : l ≤ univMax) (A_cl : A.isClosed) :
     E.snoc l c A l_le A_cl c = some ⟨(A, l), ⟨A_cl, l_le⟩⟩ := by
   simp [snoc]
 
-theorem le_snoc (E : Env χ)
+theorem le_snoc (E : Axioms χ)
     (l : Nat) (c : χ) (A : Expr χ)
     (l_le : l ≤ univMax) (A_cl : A.isClosed)
     (Ec : E c = none) :
@@ -50,33 +50,33 @@ theorem le_snoc (E : Env χ)
   have : d ≠ c := by grind
   simp only [snoc, this, ↓reduceIte, Ed]
 
-theorem _root_.of_env_le_all {E E' : Env χ} (le : E ≤ E') :
+theorem _root_.of_env_le_all {E E' : Axioms χ} (le : E ≤ E') :
     (∀ {Γ}, WfCtx E Γ → WfCtx E' Γ) ∧
     (∀ {Γ l A}, E ∣ Γ ⊢[l] A → E' ∣ Γ ⊢[l] A) ∧
     (∀ {Γ l A B}, E ∣ Γ ⊢[l] A ≡ B → E' ∣ Γ ⊢[l] A ≡ B) ∧
     (∀ {Γ l A t}, E ∣ Γ ⊢[l] t : A → E' ∣ Γ ⊢[l] t : A) ∧
     (∀ {Γ l A t u}, E ∣ Γ ⊢[l] t ≡ u : A → E' ∣ Γ ⊢[l] t ≡ u : A) := by
   mutual_induction WfCtx
-  case const =>
+  case ax =>
     intros; rename_i Ec Γ
-    apply WfTm.const Γ (le Ec)
+    apply WfTm.ax Γ (le Ec)
   grind_cases
 
-theorem Wf.snoc {E : Env χ} {A l}
+theorem Wf.snoc {E : Axioms χ} {A l}
     (Ewf : E.Wf) (c : χ) (Awf : E ∣ [] ⊢[l] A) (Ec : E c = none) :
     (E.snoc l c A Awf.le_univMax Awf.isClosed).Wf := by
   intro d Al Ed
-  simp only [Env.snoc] at Ed
+  simp only [Axioms.snoc] at Ed
   have le := E.le_snoc l c A Awf.le_univMax Awf.isClosed Ec
   by_cases eq : d = c <;> simp only [eq, ↓reduceIte] at Ed
   . cases Ed
     exact of_env_le_all le |>.2.1 Awf
   . exact of_env_le_all le |>.2.1 <| Ewf Ed
 
-end Env
+end Axioms
 
 /-- An axiom checked with respect to the axioms in `E`. -/
-structure CheckedAx (E : Env χ) where
+structure CheckedAx (E : Axioms χ) where
   name : χ
   get_name : E name = none
   l : Nat
@@ -91,7 +91,7 @@ theorem wf_tp (a : CheckedAx E) : E ∣ [] ⊢[a.l] a.tp :=
   a.wf_nfTp.wf_tp
 
 /-- The set of axioms extended by this one. -/
-noncomputable def snocEnv (a : CheckedAx E) : Env χ :=
+noncomputable def snocEnv (a : CheckedAx E) : Axioms χ :=
   E.snoc a.l a.name a.tp a.wf_tp.le_univMax a.wf_tp.isClosed
 
 theorem wf_snocEnv (a : CheckedAx E) : a.snocEnv.Wf :=
@@ -99,17 +99,17 @@ theorem wf_snocEnv (a : CheckedAx E) : a.snocEnv.Wf :=
 
 /-- The axiom as an expression. -/
 def val (a : CheckedAx E) : Expr χ :=
-  .const a.name
+  .ax a.name
 
 theorem wf_val (a : CheckedAx E) : a.snocEnv ∣ [] ⊢[a.l] a.val : a.tp := by
   unfold val
   have := E.snoc_get a.l a.name a.tp a.wf_tp.le_univMax a.wf_tp.isClosed
-  apply WfTm.const .nil this
+  apply WfTm.ax .nil this
 
 end CheckedAx
 
 /-- A definition checked with respect to the axioms in `E`. -/
-structure CheckedDef (E : Env χ) where
+structure CheckedDef (E : Axioms χ) where
   l : Nat
   tp : Expr χ
   nfTp : Val χ
