GroupoidModel/Syntax/Typechecker/Value.lean
@@ -2,7 +2,7 @@ import GroupoidModel.Syntax.GCongr
 import GroupoidModel.Syntax.Injectivity
 import GroupoidModel.Syntax.Synth
 
-variable {χ : Type*} {E : Env χ}
+variable {χ : Type*} {E : Axioms χ}
 
 /-! # Values, neutral forms, closures, and evaluation environments
 
@@ -46,7 +46,7 @@ by uniqueness of typing, lemmas like the following can be proven
 ```
 and hence it suffices to compare the value parts (in this case `p`). -/
 inductive Val where
-  | const (c : χ)
+  | ax (c : χ)
   | pi (l l' : Nat) (A : Val) (B : Clos)
   | sigma (l l' : Nat) (A : Val) (B : Clos)
   | Id (l : Nat) (A t u : Val)
@@ -96,7 +96,7 @@ end
 /-! ## Relation of values to terms -/
 
 mutual
-variable (E : Env χ)
+variable (E : Axioms χ)
 
 inductive ValEqTp : Ctx χ → Nat → Val χ → Expr χ → Prop
   | pi {Γ vA A vB B l l'} :
@@ -127,10 +127,10 @@ inductive ValEqTp : Ctx χ → Nat → Val χ → Expr χ → Prop
 -- Note: neutral types are embedded in `Val` directly and don't need a `NeutEqTp` relation.
 
 inductive ValEqTm : Ctx χ → Nat → Val χ → Expr χ → Expr χ → Prop
-  | const {Γ c Al} :
+  | ax {Γ c Al} :
     WfCtx E Γ →
     E c = some Al →
-    ValEqTm Γ Al.val.2 (.const c) (.const c) Al.val.1
+    ValEqTm Γ Al.val.2 (.ax c) (.ax c) Al.val.1
   | lam {Γ A B vA vb b l l'} :
     ValEqTp Γ l vA A →
     ClosEqTm Γ l l' A B vb b →
@@ -314,7 +314,7 @@ theorem wf_expr :
     (∀ {Γ Eᵥ σ Γ'}, EnvEqSb E Γ Eᵥ σ Γ' → WfSb E Γ σ Γ') := by
   mutual_induction ValEqTp
   all_goals dsimp; intros
-  case const => apply WfTm.const <;> assumption
+  case ax => apply WfTm.ax <;> assumption
   case conv_tp => grind [EqTp.wf_right]
   case conv_nf tt' AA' _ => exact tt'.wf_right.conv AA'
   case conv_neut nn' AA' _ => exact nn'.wf_right.conv AA'
@@ -408,7 +408,7 @@ theorem conv_ctx :
     (∀ {Γ Eᵥ σ Δ}, EnvEqSb E Γ Eᵥ σ Δ → ∀ {Γ'}, EqCtx E Γ Γ' → EnvEqSb E Γ' Eᵥ σ Δ) := by
   mutual_induction ValEqTp
   all_goals intros
-  case const => apply ValEqTm.const <;> grind [EqCtx.wf_right]
+  case ax => apply ValEqTm.ax <;> grind [EqCtx.wf_right]
   case univ => grind [ValEqTp.univ, EqCtx.wf_right]
   case pair B _ _ _ _ _ eq =>
     apply ValEqTm.pair (B.conv_ctx (eq.snoc <| EqTp.refl_tp B.wf_binder)) <;> grind
@@ -483,9 +483,9 @@ theorem wk_all :
       EnvEqSb E ((C,k) :: Γ) Eᵥ (Expr.comp Expr.wk σ) Δ) := by
   mutual_induction ValEqTp
   all_goals intros; try dsimp [Expr.subst] at *
-  case const Al _ _ _ _ _ =>
+  case ax Al _ _ _ _ _ =>
     rw [Expr.subst_of_isClosed _ Al.2.1]
-    apply ValEqTm.const <;> grind [WfCtx.snoc]
+    apply ValEqTm.ax <;> grind [WfCtx.snoc]
   case univ => grind [ValEqTp.univ, WfCtx.snoc]
   case conv_tp => grind [ValEqTp.conv_tp, EqTp.subst, WfSb.wk]
   case pair B _ _ iht ihu _ _ C =>
@@ -570,7 +570,7 @@ theorem EnvEqSb.wk {Δ Eᵥ σ Γ} (h : EnvEqSb E Δ Eᵥ σ Γ) {C k} (hC : E �
 /-- A type environment is a context where all types are in NF. -/
 abbrev TpEnv (χ) := List (Val χ × Nat)
 
-variable (E : Env χ) in
+variable (E : Axioms χ) in
 inductive TpEnvEqCtx : TpEnv χ → Ctx χ → Prop
   | nil : TpEnvEqCtx [] []
   | snoc {vΓ Γ l vA A} :
